Write introduction and explain representation.

theories/Reflection.v
@@ -1,3 +1,4 @@
+(* begin hide *)
 Require Import Ssreflect.ssreflect Ssreflect.ssrfun Ssreflect.ssrbool.
 Require Import Ssreflect.ssrnat Ssreflect.eqtype Ssreflect.seq.
 Require Import MathComp.bigop MathComp.path.
@@ -5,41 +6,180 @@ Require Import MathComp.bigop MathComp.path.
 Set Implicit Arguments.
 Unset Strict Implicit.
 Unset Printing Implicit Defensive.
+(* end hide *)
+(** One important aspect of Coq's logic is the special status it gives
+to _computation_: while some systems require one to apply explicit
+reasoning steps to show that two given terms are equal, Coq's logic
+considers any two terms that _evaluate_ to the same result to be equal
+automatically, without the need for additional reasoning steps.
+
+Without getting into too much detail, we can illustrate this idea with
+some simple examples. Russell and Whitehead's seminal _Principia
+Mathematica_ had to develop #<a
+href="http://quod.lib.umich.edu/cgi/t/text/pageviewer-idx?c=umhistmath&cc=umhistmath&idno=aat3201.0001.001&frm=frameset&view=image&seq=401">hundreds
+of pages</a># of foundational mathematics before being able to prove
+that [1 + 1 = 2]. In contrast, here's what this proof looks like in
+Coq: *)
+
+Definition one_plus_one : 1 + 1 = 2 := erefl.
+
+(** [erefl] is the only constructor of the [eq] type; its type,
+[forall A (a : A), a = a], tells us that we can use it to prove that
+given term [a] is equal to itself. Coq accepts this proof because,
+even though the two sides of the equation are not syntactically the
+same, it is able to use the definition of [+] to compute the left-hand
+side and check that the result is the same as the right-hand
+side. This also works for some statements with variables in them, for
+instance *)
+
+Definition zero_plus_n n : 0 + n = n := erefl.
+
+(** The same principle applies here: [+] is defined by case analysis
+on its first argument, and doesn't even need to inspect the second
+one. Since the first argument on the left-hand side is a constructor
+([0]), Coq can use this definition to reduce it to [n].
+
+Unfortunately, not every equality is a direct consequence of
+computation. For example, this proof attempt is rejected: *)
+
+Fail Definition n_plus_zero n : n + 0 = n := erefl.
+
+(** What happened here? As mentioned before, [+] is defined by case
+analysis on the first argument; since the first argument of the
+left-hand side doesn't start with a constructor, Coq doesn't know how
+to compute there. As it turns out, one actually needs an inductive
+argument to prove this result, which might end up looking like this,
+if we were to check the proof term that Coq produces: *)
+
+Fixpoint n_plus_zero n : n + 0 = n :=
+  match n with
+  | 0 => erefl
+  | n.+1 => let: erefl := n_plus_zero n in erefl
+  end.
+
+(** It seems that, although interesting, computation inside Coq isn't
+of much use when proving something. Or is it?
+
+In this post, I will show how computation in Coq can be used to write
+certified tactics for automating certain reasoning steps. This
+technique, known as _proof by reflection_, played an important role in
+the Coq formalization of the #<a
+href="http://en.wikipedia.org/wiki/Four_color_theorem">Four-color
+theorem</a>#, and has been used for many other developments, even in
+other proof assistants. As a matter of fact, the name #<a
+href="http://ssr.msr-inria.inria.fr/">Ssreflect</a># stands for
+_small-scale reflection_, due to the pervasive use of reflection and
+computation. Let's see how reflection works by means of a basic (but
+interesting) example: a tactic for checking equalities between simple
+expressions involving natural numbers.
+
+** Arithmetic with reflection
+
+Imagine that we were in the middle of a proof and needed to show that
+two natural numbers are equal: *)
+
+Lemma lem n m p : (n + m) * (2 ^ p) = (2 ^ p) * m + (2 ^ p) * n.
+
+(** This lemma is simple enough so that Coq's own [ring] tactic can
+solve it automatically for us, but just for the sake of the example,
+suppose that we had to prove this by hand. We could write something
+like *)
+
+Proof. by rewrite mulnDl (mulnC n) (mulnC m) addnC. Qed.
+
+(** This was not terribly complicated, but there's certainly room for
+improvement. In a paper proof, a mathematician would probably assume
+that the reader would be able to verify this result on their own,
+without needing any additional detail. But how exactly would the
+reader proceed?
+
+In the case of the simple arithmetic expression above, one strategy is
+to apply the distributivity law as long as we can, until both
+expressions become a sum of monomials. Then, thanks to associativity
+and commutativity, we just have to reorder the factors and terms and
+check that both sides of the equation match.
+
+The idea of proof by reflection is to reduce a the validity of a
+logical statement to a _symbolic computation_, usually by proving a
+theorem of the form [thm : b = true -> P] with [b : bool]. If [b] can
+be computed explicitly and reduces to [true], then Coq recognizes
+[erefl] as a proof of [b = true], which means that [thm erefl] becomes
+a proof of [P].
+
+To make things concrete, let's go back to our example. The idea that
+we described above for checking whether two numbers are equal can be
+used whenever we have expressions involving addition, multiplication,
+and variables. We will define a Coq data type for representing such
+expressions, as we will need to compute with them: *)
 
 Inductive expr :=
 | Var of nat
 | Add of expr & expr
 | Mul of expr & expr.
 
-Fixpoint nat_of_expr vm e :=
+(** Variables are represented by natural numbers using the [Var]
+constructor, and we can add and multiply expressions together with the
+[Add] and [Mul] constructors. The following term, for instance,
+represents the expression [n + (m * n)]: *)
+
+Example expr_ex :=
+  Add (Var 0) (Mul (Var 1) (Var 0)).
+
+(** where [Var 0] and [Var 1] denote [n] and [m], respectively.
+
+If we are given a function [vals] assigning variables to numbers, we
+can compute the value of an expression with a simple recursive
+function: *)
+
+Fixpoint nat_of_expr vals e :=
   match e with
-  | Var v => nth 0 vm v
-  | Add e1 e2 => nat_of_expr vm e1 + nat_of_expr vm e2
-  | Mul e1 e2 => nat_of_expr vm e1 * nat_of_expr vm e2
+  | Var v => vals v
+  | Add e1 e2 => nat_of_expr vals e1 + nat_of_expr vals e2
+  | Mul e1 e2 => nat_of_expr vals e1 * nat_of_expr vals e2
   end.
 
-Fixpoint normalize_int e :=
+(** Now, we know that every expression of that form can be written as
+a sum of monomials. We can then define a function [monoms] for
+converting an [expr] to that form: *)
+
+Fixpoint monoms e :=
   match e with
   | Var v => [:: [:: v]]
-  | Add e1 e2 => normalize_int e1 ++ normalize_int e2
-  | Mul e1 e2 => allpairs cat (normalize_int e1) (normalize_int e2)
+  | Add e1 e2 => monoms e1 ++ monoms e2
+  | Mul e1 e2 => allpairs cat (monoms e1) (monoms e2)
   end.
 
-Definition normalize := map (sort leq) \o normalize_int.
+(** Here, we represent a sum of monomials with a list of lists of
+variable numbers; for example, here's the result of normalizing
+[expr_ex]: *)
 
-Lemma normalizeE vm e :
-  nat_of_expr vm e = \sum_(s <- normalize e) \prod_(n <- s) nth 0 vm n.
+Example monoms_expr_ex :
+  monoms expr_ex = [:: [:: 0]; [:: 1; 0]].
+Proof. by []. Qed.
+
+(** (The [allpairs] function in the body of [monoms] comes from
+the [seq] Ssreflect library, and outputs all possible combinations of
+elements of two given lists using some binary function (in this case,
+list concatenation)). *)
+
+Lemma monomsE vals e :
+  nat_of_expr vals e = \sum_(m <- monoms e) \prod_(v <- m) vals v.
 Proof.
-transitivity (\sum_(s <- normalize_int e) \prod_(n <- s) nth 0 vm n).
-  elim: e=> [v|e1 IH1 e2 IH2|e1 IH1 e2 IH2] /=.
-  - by rewrite 2!big_seq1.
-  - by rewrite big_cat IH1 IH2.
-  rewrite {}IH1 {}IH2 big_distrlr /=.
-  elim: (normalize_int e1) (normalize_int e2)=> [|v s1 IH] s2 /=.
-    by rewrite 2!big_nil.
-  rewrite big_cons big_cat /= IH; congr addn.
-  by rewrite big_map; apply/eq_big=> //= s3 _; rewrite big_cat.
-rewrite /normalize /=; elim: (normalize_int e)=> [|s ss IH] /=.
+elim: e=> [v|e1 IH1 e2 IH2|e1 IH1 e2 IH2] /=.
+- by rewrite 2!big_seq1.
+- by rewrite big_cat IH1 IH2.
+rewrite {}IH1 {}IH2 big_distrlr /=.
+elim: (monoms e1) (monoms e2)=> [|v m1 IH] m2 /=; first by rewrite 2!big_nil.
+rewrite big_cons big_cat /= IH; congr addn.
+by rewrite big_map; apply/eq_big=> //= m3 _; rewrite big_cat.
+Qed.
+
+Definition normalize := map (sort leq) \o monoms.
+
+Lemma normalizeE vals e :
+  nat_of_expr vals e = \sum_(m <- normalize e) \prod_(v <- m) vals v.
+Proof.
+rewrite monomsE /normalize /=; elim: (monoms e)=> [|m ms IH] /=.
   by rewrite big_nil.
 rewrite 2!big_cons IH; congr addn.
 by apply/eq_big_perm; rewrite perm_eq_sym perm_sort.
@@ -98,15 +238,10 @@ Ltac quote_eq :=
     | (?qe1, ?vm') =>
       let r2 := quote_expr vm' e2 in
       match r2 with
-      | (?qe2, ?vm'') => apply (@expr_eqP vm'' qe1 qe2 erefl)
+      | (?qe2, ?vm'') => apply (@expr_eqP (nth 0 vm'') qe1 qe2 erefl)
       end
     end
   end.
-
-Lemma l1 n m p : (n + m) * (2 ^ p) = (2 ^ p) * m + (2 ^ p) * n.
-Proof.
-by rewrite mulnDl (mulnC n) (mulnC m) addnC.
-Qed.
 
 Lemma l1' n m p : (n + m) * (2 ^ p) = (2 ^ p) * m + (2 ^ p) * n.
 Proof. quote_eq. Qed.
